# 1.1 - Brief Review of Differentiation

## Definition of the Derivative

$f : R \to R$ is differentiable at $x \in R$ if the limit

$$ lim_{h \to 0} = \frac{f(x+h)-f(x)}{h}$$

exists, in which case the derivate $ f'(x) $ is

$$ f'(x) = lim_{h \to 0} = \frac{f(x+h)-f(x)}{h}$$

### Theorem 1.1 (Product Rule)

The product $ f(x)g(x) $ of two differentiable functions $ f(x) $ and $ g(x) $ is differentiable, and

$$ (f(x)g(x))' = f'(x)g(x) + f(x)g'(x) $$

### Theorem 1.2 (Quotient Rule)

The quotient $ \frac{f(x)}{g(x)} $ of two differentiable functions $ f(x) $ and $ g(x) $ is differentiable at every point $ x $ where the function $ \frac{f(x)}{g(x)} $ is well-defined and

$$ \left(\frac{f(x)}{g(x)}\right)' = \frac{f'(x)g(x) - f(x)g'(x)}{(g(x))^2}$$

### Theorem 1.3 (Chain Rule)

The composite function $ (g \circ f)(x) = g(f(x)) $ of two differentiable functions $ f(x) $ and $ g(x) $ is differentiable at every point $ x $ where $ g(f(x)) $ is well-defined and

$$ (g(f(x)))' = g'(f(x)) f'(x) $$

The Chain Rule formula can also be written as

$$ \frac{dg}{dx} = \frac{dg}{du}\frac{du}{dx'} $$

where $ u = f(x) $ is a function of $ x $ and $ g = g(u) = g(f(x)) $.

This rule is often used for power functions, exponential functions and logarithmic functions:

$$ \frac{d}{dx}((f(x)^n) = n(f(x))^{n-1} f'(x) $$

$$ \frac{d}{dx}(e^{f(x)}) = e^{f(x)} f'(x) $$

$$ \frac{d}{dx}(\ln f(x)) = \frac{f'(x)}{f(x)} $$

#### Lemma 1.1 (Derivative of Inverse Function)

Let $ f : [a, b] \to [c, d] $ be a differentiable function, and assume that $ f(x) $ has an inverse function denoted by $ f^{-1}(x) $, with $ f^{-1} : [c, d] \to [a, b] $. The function $ f^{-1}(x) $ is differentiable at every point $ x \in [c, d] $ where $ f'(f^{-1}(x)) \neq 0 $ and

$$ (f^{-1}(x))' = \frac{1}{f'(f^{-1}(x))} $$

The above formula is derived from the Chain Rule:

$$ (g(f(z)))' = g'(f(z)) f'(z) $$

Let $ g = f^{-1} $. Since $ g(f(z)) = f^{-1}(f(z)) = z $, it follows that

$$ 1 = (f^{-1})'(f(z))\cdot f'(z) $$

Let $ z = f^{-1}(x) \neq 0 $, then $ f(z) = f(f^{-1}(x)) = x $ and

$$ 1 = (f^{-1})'(x)\cdot f'(f^{-1}(x)) = (f^{-1}(x))'\cdot f'(f^{-1}(x))$$

If $ f'(f^{-1}(x)) \neq 0 $, then we can simplify both sides to yield the original formula.
