# 1.5 - L'H么pital's Rule and Connections to Taylor Expansions

## Definition

This rule is used to compute limits when direct computation would yield and undefined result of the form $\frac{0}{0}$. If $\lim_{x\to x_0}f(x) = \lim_{x\to x_0}g(x) = 0$, and if $\lim_{x\to x_0}\frac{f'(x)}{g'(x)}$ exists, then $\lim_{x\to x_0}\frac{f(x)}{g(x)}$ exists and $\lim_{x\to x_0}\frac{f(x)}{g(x)} = \lim_{x\to x_0}\frac{f'(x)}{g'(x)}$.

### Theorem 1.8

Let $x_0$ be a real number; allow $x_0 = \infty$ and $x_0 = -\infty$. Let $f(x)$ and $g(x)$ be two differentiable functions.

1. Assume that $\lim_{x\to x_0}f(x) = 0$ and  $\lim_{x\to x_0}g(x) = 0$. If $\lim_{x\to x_0}\frac{f'(x)}{g'(x)}$ exists, and if there exists an interval $(a, b)$ around $x_0$ such that $g'(x) \neq 0$ for all $x \in (a, b) \setminus 0$, then the limit $\lim_{x\to x_0}\frac{f(x)}{g(x)}$ also exists, and

$$ \lim_{x\to x_0}\frac{f(x)}{g(x)} = \lim_{x\to x_0}\frac{f'(x)}{g'(x)} $$

2. Assume that $\lim_{x\to x_0}f(x)$ is either $-\infty$ or $\infty$ and that $\lim_{x\to x_0}g(x)$ is either $-\infty$ or $\infty$. If the limit $\lim_{x\to x_0}\frac{f'(x)}{g'(x)}$ exists, and if there exists an interval $(a, b)$ around $x_0$ such that $g'(x) \neq 0$ for all $x \in (a, b) \setminus 0$, then the limit $\lim_{x\to x_0}\frac{f(x)}{g(x)}$ also exists and

$$ \lim_{x\to x_0}\frac{f(x)}{g(x)} = \lim_{x\to x_0}\frac{f'(x)}{g'(x)} $$

If $x_0 = - \infty$ or if $x_0 = \infty$, the interval $(a, b)$ from [Theorem 1.8](#theorem-18) is of the form $(-\infty, b)$ and $(a, \infty)$ respectively. This rule can also be applied to other undefined limits such as

$$ 0 \cdot \infty,\quad \frac{1}{0\cdot\infty},\quad 0^0,\quad \infty^0,\quad 1^\infty $$

Furthermore, l'H么pital's rule can be used to prove [Taylor Expansions](https://mathworld.wolfram.com/TaylorSeries.html) hold true on small intervals. For example, the linear expansion of the function $e^x$ around the point $0$ is $e^x \approx 1 + x$. Using l'H么pital's rule, we can show that

$$ lim_{x\to 0}\frac{e^x - (1+x)}{x^2} = \frac{1}{2} $$

We first differentiate both the numerator and denominator and obtain the following limit

$$ \lim_{x\to 0} \frac{e^x - 1}{2x} $$

This limit is $\frac{0}{0}$. Therefore, apply l'H么pital's rule again by differentiating the numerator and denominator;

$$ \lim_{x\to 0}\frac{e^x}{2} = \frac{1}{2} $$

We conclude that

$$ lim_{x\to 0}\frac{e^x - (1+x)}{x^2} = \frac{1}{2} $$
